comm/JITCall.v
@@ -2,7 +2,7 @@ From compcert Require Import Memory Memtype Integers Values Ctypes AST.
 From compcert.arm Require Import AsmSyntax ABinSem.
 From Coq Require Import ZArith Lia List.
 
-From bpf.comm Require Import Regs ListAsArray.
+From bpf.comm Require Import Regs ListAsArray rBPFMemType.
 
 Open Scope Z_scope.
 Import ListNotations.
@@ -11,14 +11,16 @@ Definition JITTED_LIST_MAX_LENGTH: nat := 4000.
 
 (**r input: jitted_start_addr -> jit_state_start_addr -> result *)
 Definition compcertbin_signature: signature :=
-  {| sig_args := [AST.Tint; AST.Tint]; sig_res := AST.Tint; sig_cc := cc_default |}.
+  {| sig_args := [AST.Tint; AST.Tint]; sig_res := AST.Tint; sig_cc :=
+    {| AST.cc_vararg := Some 1%Z; AST.cc_unproto := false; AST.cc_structret := false |} |}.
 
 
 
 Definition state_block_size: Z := 52.
 Definition stack_block_size: Z := 48.
 
-Axiom jit_arm_start_address : val.
+Axiom jit_arm_block : block.
+Axiom jit_state_block : block.
 
 Definition get_result_bool (r:rettype) (v:aval): bool :=
   match v with
@@ -26,41 +28,46 @@ Definition get_result_bool (r:rettype) (v:aval): bool :=
   | _     => false
   end.
 
+Definition store_vint (chunk: memory_chunk) (m: mem) (b: block) (ofs: Z) (v: val): option mem :=
+  match v with
+  | Vint vi => Mem.store chunk m b ofs v
+  | _ => None
+  end.
 
 Definition rbpf_copy_to (pc: int) (rs: regmap) (st_blk: block) (m: mem): option mem :=
-  match Mem.store Mint32 m st_blk   0   (eval_regmap R0  rs) with
+  match store_vint Mint32 m st_blk   0   (eval_regmap R0  rs) with
   | None => None
   | Some m0 =>
-  match Mem.store Mint32 m0 st_blk  4   (eval_regmap R1  rs) with
+  match store_vint Mint32 m0 st_blk  4   (eval_regmap R1  rs) with
   | None => None
   | Some m1 =>
-  match Mem.store Mint32 m1 st_blk  8   (eval_regmap R2  rs) with
+  match store_vint Mint32 m1 st_blk  8   (eval_regmap R2  rs) with
   | None => None
   | Some m2 =>
-  match Mem.store Mint32 m2 st_blk  12  (eval_regmap R3  rs) with
+  match store_vint Mint32 m2 st_blk  12  (eval_regmap R3  rs) with
   | None => None
   | Some m3 =>
-  match Mem.store Mint32 m3 st_blk  16  (eval_regmap R4  rs) with
+  match store_vint Mint32 m3 st_blk  16  (eval_regmap R4  rs) with
   | None => None
   | Some m4 =>
-  match Mem.store Mint32 m4 st_blk  20  (eval_regmap R5  rs) with
+  match store_vint Mint32 m4 st_blk  20  (eval_regmap R5  rs) with
   | None => None
   | Some m5 =>
-  match Mem.store Mint32 m5 st_blk  24  (eval_regmap R6  rs) with
+  match store_vint Mint32 m5 st_blk  24  (eval_regmap R6  rs) with
   | None => None
   | Some m6 =>
-  match Mem.store Mint32 m6 st_blk  28  (eval_regmap R7  rs) with
+  match store_vint Mint32 m6 st_blk  28  (eval_regmap R7  rs) with
   | None => None
   | Some m7 =>
-  match Mem.store Mint32 m7 st_blk  32  (eval_regmap R8  rs) with
+  match store_vint Mint32 m7 st_blk  32  (eval_regmap R8  rs) with
   | None => None
   | Some m8 =>
-  match Mem.store Mint32 m8 st_blk  36  (eval_regmap R9  rs) with
+  match store_vint Mint32 m8 st_blk  36  (eval_regmap R9  rs) with
   | None => None
   | Some m9 =>
-  match Mem.store Mint32 m9 st_blk  40  (eval_regmap R10  rs) with
+  match store_vint Mint32 m9 st_blk  40  (eval_regmap R10  rs) with
   | None => None
-  | Some m10 => Mem.store Mint32 m10 st_blk 44 (Vint pc)
+  | Some m10 => store_vint Mint32 m10 st_blk 44 (Vint pc)
   end
   end
   end
@@ -73,41 +80,47 @@ Definition rbpf_copy_to (pc: int) (rs: regmap) (st_blk: block) (m: mem): option 
   end
   end.
 
+Definition load_vint (chunk: memory_chunk) (m: mem) (b: block) (ofs: Z): option val :=
+  match Mem.load chunk m b ofs with
+  | Some (Vint vi) => Some (Vint vi)
+  | _ => None
+  end.
+
 Definition rbpf_copy_from (rs: regmap) (st_blk: block) (m: mem): option (val * regmap) :=
-  match Mem.load Mint32 m st_blk 0 with
+  match load_vint Mint32 m st_blk 0 with
   | None => None
   | Some v0 =>
-  match Mem.load Mint32 m st_blk 4 with
+  match load_vint Mint32 m st_blk 4 with
   | None => None
   | Some v1 =>
-  match Mem.load Mint32 m st_blk 8  with
+  match load_vint Mint32 m st_blk 8  with
   | None => None
   | Some v2 =>
-  match Mem.load Mint32 m st_blk 12 with
+  match load_vint Mint32 m st_blk 12 with
   | None => None
   | Some v3 =>
-  match Mem.load Mint32 m st_blk 16 with
+  match load_vint Mint32 m st_blk 16 with
   | None => None
   | Some v4 =>
-  match Mem.load Mint32 m st_blk 20 with
+  match load_vint Mint32 m st_blk 20 with
   | None => None
   | Some v5 =>
-  match Mem.load Mint32 m st_blk 24 with
+  match load_vint Mint32 m st_blk 24 with
   | None => None
   | Some v6 =>
-  match Mem.load Mint32 m st_blk 28 with
+  match load_vint Mint32 m st_blk 28 with
   | None => None
   | Some v7 =>
-  match Mem.load Mint32 m st_blk 32 with
+  match load_vint Mint32 m st_blk 32 with
   | None => None
   | Some v8 =>
-  match Mem.load Mint32 m st_blk 36 with
+  match load_vint Mint32 m st_blk 36 with
   | None => None
   | Some v9 =>
-  match Mem.load Mint32 m st_blk 40 with
+  match load_vint Mint32 m st_blk 40 with
   | None => None
   | Some v10 =>
-  match Mem.load Mint32 m st_blk 44 with
+  match load_vint Mint32 m st_blk 44 with
   | None => None
   | Some vpc =>
     Some (vpc,
@@ -139,29 +152,59 @@ Definition rbpf_copy_from (rs: regmap) (st_blk: block) (m: mem): option (val * r
 Definition jit_call_simpl (ofs: nat) (pc: int) (rs: regmap) (m: mem): option (int * regmap * mem) :=
   let fuel  := JITTED_LIST_MAX_LENGTH in
   let sz    := (Int.repr stack_block_size) in (**r 12 * 4 *)
-    let (m1, st_blk) := Mem.alloc m 0 state_block_size in
-      match rbpf_copy_to pc rs st_blk m1 with
-      | None => None
-      | Some m2 =>
-        let jitted_arm_address := Val.add jit_arm_start_address
-          (Vint (Int.repr (Z.of_nat (Nat.mul 4 ofs)))) (*
-          (Vint (Int.mul (Int.repr (Z.of_nat ofs)) (Int.repr 2))) *) in
-        let arm_argu_list_val := [jitted_arm_address; (Vptr st_blk Ptrofs.zero)] in
-          match bin_exec fuel compcertbin_signature (Int.unsigned sz)
-            Ptrofs.zero arm_argu_list_val m2 with
+    match rbpf_copy_to pc rs jit_state_block m with
+    | None => None
+    | Some m2 =>
+      let arm_argu_list_val :=
+        [ (Vptr jit_arm_block (Ptrofs.mul (Ptrofs.repr 4)
+            (Ptrofs.of_intu (Int.repr (Z.of_nat ofs)))));
+          (Vptr jit_state_block Ptrofs.zero)] in
+        match bin_exec fuel compcertbin_signature (Int.unsigned sz)
+          Ptrofs.zero arm_argu_list_val m2 with
+        | None => None
+        | Some (_, m3) =>
+          match rbpf_copy_from rs jit_state_block m3 with
           | None => None
-          | Some (_, m3) =>
-            match rbpf_copy_from rs st_blk m3 with
-            | None => None
-            | Some (vpc, rs') =>
-              match vpc with
-              | Vint pc' => Some (pc', rs', m) (*
-                match Mem.free m3 st_blk 0 state_block_size with
-                | None => None
-                | Some m' => Some (pc', rs', m')
-                end *)
-              | _ => None
-              end
+          | Some (vpc, rs') =>
+            match vpc with
+            | Vint pc' => Some (pc', rs', m) (*
+              match Mem.free m3 st_blk 0 state_block_size with
+              | None => None
+              | Some m' => Some (pc', rs', m')
+              end *)
+            | _ => None
             end
           end
-      end.
+        end
+    end.
+
+Lemma store_vint_unchanged_on:
+  forall chunk m1 st_blk ofs v m2 m (P: block -> Z -> Prop)
+    (Hstore : store_vint chunk m1 st_blk ofs v = Some m2)
+    (Hblk_neq: forall ofs, ~P st_blk ofs)
+    (munchange : Mem.unchanged_on P m1 m),
+      Mem.unchanged_on P m2 m.
+Proof.
+  unfold store_vint.
+  intros.
+  destruct v; inversion Hstore.
+  clear H0.
+  eapply store_unchanged_on_4; eauto.
+Qed.
+
+Lemma rbpf_copy_to_unchanged_on:
+  forall pc rs st_blk m1 m2 m (P: block -> Z -> Prop)
+    (Hcopy_to : rbpf_copy_to pc rs st_blk m1 = Some m2)
+    (Hblk_neq: forall ofs, ~P st_blk ofs)
+    (munchange : Mem.unchanged_on P m1 m),
+      Mem.unchanged_on P m2 m.
+Proof.
+  unfold rbpf_copy_to.
+  intros.
+  repeat (destruct store_vint eqn: Hn_eq; [
+    eapply store_vint_unchanged_on in Hn_eq; eauto;
+    clear munchange; rename Hn_eq into munchange |
+    inversion Hcopy_to ]).
+  inversion Hcopy_to.
+  subst m2; auto.
+Qed.
