jit/simulation/correct_get_src32.v
@@ -1,34 +1,15 @@
-(**************************************************************************)
-(*  This file is part of CertrBPF,                                        *)
-(*  a formally verified rBPF verifier + interpreter + JIT in Coq.         *)
-(*                                                                        *)
-(*  Copyright (C) 2022 Inria                                              *)
-(*                                                                        *)
-(*  This program is free software; you can redistribute it and/or modify  *)
-(*  it under the terms of the GNU General Public License as published by  *)
-(*  the Free Software Foundation; either version 2 of the License, or     *)
-(*  (at your option) any later version.                                   *)
-(*                                                                        *)
-(*  This program is distributed in the hope that it will be useful,       *)
-(*  but WITHOUT ANY WARRANTY; without even the implied warranty of        *)
-(*  MERCHANTABILITY or FITNESS FOR A PARTICULAR PURPOSE.  See the         *)
-(*  GNU General Public License for more details.                          *)
-(*                                                                        *)
-(**************************************************************************)
-
-From bpf.comm Require Import Regs State Monad.
-From bpf.monadicmodel Require Import rBPFInterpreter.
 From Coq Require Import List Lia ZArith.
 From compcert Require Import Coqlib Integers Values Clight Memory.
 Import ListNotations.
 
 From bpf.clightlogic Require Import Clightlogic CorrectRel CommonLemma.
 
-From bpf.clight Require Import interpreter.
+From bpf.jit.jitclight Require Import havm_interpreter.
+From bpf.jit.havm Require Import HAVMState HAVMMonadOp DxHAVMInterpreter.
 
-From bpf.simulation Require Import MatchState InterpreterRel.
+From bpf.jit.simulation Require Import MatchStateComm HAVMMatchState InterpreterRel.
 
-From bpf.simulation Require Import correct_get_immediate correct_get_src correct_eval_reg.
+From bpf.jit.simulation Require Import correct_get_immediate correct_get_src correct_eval_reg.
 
 
 (**
@@ -52,7 +33,7 @@ Section Get_src32.
   Definition res : Type := (val:Type).
 
   (* [f] is a Coq Monadic function with the right type *)
-  Definition f : arrow_type args (M State.state res) := get_src32.
+  Definition f : arrow_type args (M res) := get_src32.
 
   (* [fn] is the Cligth function which has the same behaviour as [f] *)
   Definition fn: Clight.function := f_get_src32.
@@ -65,7 +46,7 @@ Section Get_src32.
                     (DList.DNil _))).
 
   (* [match_res] relates the Coq result and the C result *)
-  Definition match_res : res -> Inv State.state := fun x  => StateLess _ (val32_correct x).
+  Definition match_res : res -> Inv hybrid_state := fun x  => StateLess _ (val32_correct x).
 
   Instance correct_function_get_src32 : forall a, correct_function _ p args res f fn ModNothing false match_state match_arg_list match_res a.
   Proof.
@@ -75,9 +56,10 @@ Section Get_src32.
     unfold INV.
     unfold f, cl_app, get_src32.
     intros.
+    
 
     correct_forward.
-    -
+    - unfold bindM, returnM.
       correct_forward.
 
       get_invariant _ins.
@@ -102,7 +84,7 @@ Section Get_src32.
       { subst. reflexivity. }
       {simpl ; auto.
       }
-    -
+    - unfold bindM.
       correct_forward.
 
       get_invariant _ins.
@@ -127,10 +109,10 @@ Section Get_src32.
         unfold eval_inv, correct_get_src.match_res in *.
         tauto.
       }
-      intros.
+      intros. unfold returnM.
       correct_forward.
 
-      get_invariant _src32.
+      get_invariant _v.
       destruct c1 as (Hv_eq & vl & Hvl_eq).
       subst.
       eexists. split_and.
