jit/simulation/correct_jit_call.v
@@ -40,6 +40,31 @@ Definition match_arg_list : DList.t (fun x => x -> Inv _) ((unit:Type) ::args) :
   (* [match_res] relates the Coq result and the C result *)
   Definition match_res : res -> Inv hybrid_state := fun _  => StateLess _ (fun v => v = Vundef).
 
+(*
+
+Axiom bin_exec_mem_inv1:
+  forall fuel sg sz ofs lv m1 m2 res,
+    ABinSem.bin_exec fuel sg sz ofs lv m1 = Some (res, m2) -> m1 = m2.
+
+Axiom bin_exec_mem_inv2:
+  forall fuel sg sz ofs lv m1 m2 m1' res P,
+    ABinSem.bin_exec fuel sg sz ofs lv m1 = Some (res, m1') ->
+    Mem.unchanged_on P m1 m2 ->
+    exists m2',
+    ABinSem.bin_exec fuel sg sz ofs lv m2 = Some (res, m2') /\
+    Mem.unchanged_on P m1' m2'. *)
+
+Axiom bin_exec_mem_inv:
+  forall fuel sg sz ofs lv m m3 m4 res st pc1 rs1
+    (MS : match_state st m)
+    (Hcopy_to : rbpf_copy_to (pc_loc st) (regs_st st) jit_state_block (bpf_m st) = Some m3)
+    (Hbin : ABinSem.bin_exec fuel sg sz ofs lv m3 = Some (res, m4))
+    (Hcopy_from : rbpf_copy_from (regs_st st) jit_state_block m4 = Some (Vint pc1, rs1)),
+      exists m',
+        ABinSem.bin_exec fuel sg sz ofs lv m = Some (res, m') /\
+        match_state (upd_mem (bpf_m st) (upd_regs rs1 (HAVMState.upd_pc pc1 st))) m'.
+
+
   Instance correct_function_upd_reg : forall a, correct_function _ p args res f fn modifies false match_state match_arg_list match_res a.
   Proof.
     correct_function_from_body args.
@@ -53,18 +78,339 @@ Definition match_arg_list : DList.t (fun x => x -> Inv _) ((unit:Type) ::args) :
     destruct ListKeyV.index eqn: Hnth; [| auto].
     destruct jit_call_simpl as [((pc1 & rs1) & m1) |] eqn: Hcall; [| auto].
     intros.
-    exists Vundef, m1, Events.E0.
 
     unfold jit_call_simpl in Hcall.
-    destruct Mem.alloc as (m2 & st_blk2) eqn: Halloc.
     destruct rbpf_copy_to as [m3 |] eqn: Hcopy_to; [| inversion Hcall].
     destruct ABinSem.bin_exec as [(res & m4)|] eqn: Hbin; [| inversion Hcall].
     destruct rbpf_copy_from as [(pc2 & rs2)|] eqn: Hcopy_from; [| inversion Hcall].
     destruct pc2; inversion Hcall; subst; clear Hcall.
 
-    unfold state_block_size in Halloc.
+    set (HST := MS).
+    destruct HST.
+    simpl in mpc.
+    simpl in mkv.
+    destruct mkv as (Hload_kv & Hkv).
+    unfold match_kv in Hkv.
+    destruct Hkv as (Hkv_len & Hkv_max & Hkv).
+    unfold match_list_kv in Hkv.
+    destruct mbin as (Hload_bin & mbin & Heq1 & Heq2).
+    eapply bin_exec_mem_inv in Hbin as Hm_eq; eauto.
+    destruct Hm_eq as (m' & Hbin1 & Hst1).
+
+    assert (Hmem_unchanged_on_m3_m: Mem.unchanged_on (fun b _ =>
+               b <> st_blk /\ b <> mrs_blk /\ b <> ins_blk /\ b <> jit_blk /\ b <> kv_blk) m3 m). {
+      eapply rbpf_copy_to_unchanged_on with (m := m) in Hcopy_to; eauto.
+      intros ofs HF.
+      destruct HF as (HF & _).
+      apply HF.
+      auto.
+    }
+
+    unfold ListKeyV.index in Hnth.
+    specialize (Hkv (Z.to_nat (Int.unsigned (pc_loc st)))).
+    assert (Hr: (0 <= Z.to_nat (Int.unsigned (pc_loc st)) < length (tp_kv st))%nat).
+    {
+      clear - Hnth.
+      split; [lia | ].
+      eapply nth_error_Some; eauto.
+      intro HF.
+      rewrite HF in Hnth.
+      inversion Hnth.
+    }
+    specialize (Hkv Hr).
+    destruct Hkv as (Hkv1 & Hkv2).
+    unfold Mem.loadv in Hkv1.
+    assert (Heq:
+    (Ptrofs.unsigned (Ptrofs.repr (8 * Z.of_nat (Z.to_nat (Int.unsigned (pc_loc st)))))) =
+    (Ptrofs.unsigned (Ptrofs.mul (Ptrofs.repr 8) (Ptrofs.of_intu (pc_loc st))))). {
+      clear - Hr.
+      f_equal.
+      unfold Ptrofs.mul, Ptrofs.of_intu, Ptrofs.of_int.
+      f_equal.
+      change (Ptrofs.unsigned (Ptrofs.repr 8)) with 8%Z.
+      rewrite Ptrofs.unsigned_repr_eq.
+      change Ptrofs.modulus with Int.modulus.
+      rewrite <- Int.unsigned_repr_eq.
+      rewrite Int.repr_unsigned.
+      rewrite Z2Nat.id.
+      f_equal.
+      set (Int_unsigned_ge_zero (pc_loc st)) as Heq. lia.
+    }
+    rewrite Heq in Hkv1; clear Heq.
+
+    unfold Mem.loadv in Hkv2.
+    assert (Heq: (Ptrofs.unsigned (Ptrofs.repr (8 * Z.of_nat (Z.to_nat (Int.unsigned (pc_loc st))) + 4))) = (Ptrofs.unsigned
+(Ptrofs.add (Ptrofs.mul (Ptrofs.repr 8) (Ptrofs.of_intu (pc_loc st))) (Ptrofs.repr 4)))). {
+      clear - Hr Hkv_len Hkv_max.
+      f_equal.
+      unfold Ptrofs.add, Ptrofs.mul, Ptrofs.of_intu, Ptrofs.of_int.
+      f_equal.
+      change (Ptrofs.unsigned (Ptrofs.repr 8)) with 8%Z.
+      change (Ptrofs.unsigned (Ptrofs.repr 4)) with 4%Z.
+      repeat rewrite Ptrofs.unsigned_repr_eq.
+      change Ptrofs.modulus with Int.modulus.
+      repeat rewrite <- Int.unsigned_repr_eq.
+      set (Int_unsigned_ge_zero (pc_loc st)) as Heq.
+      rewrite Int.repr_unsigned.
+      rewrite Z2Nat.id; try lia.
+      rewrite Int.unsigned_repr.
+      - f_equal.
+      - change Int.max_unsigned with Ptrofs.max_unsigned.
+          rewrite Hkv_len in *.
+          change  Ptrofs.max_unsigned with 4294967295%Z in *.
+          split; lia.
+    }
+    rewrite Heq in Hkv2; clear Heq.
+(*
+    assert (Hstore_m:
+      exists mk, Mem.store AST.Mint32 m st_blk (Ptrofs.unsigned (Ptrofs.repr 44))
+  (Vint (Int.add (pc_loc st) (Int.repr (Z.of_nat (alu32_ofs k))))) = Some mk). {
+      assert (Heq: Mem.valid_access m AST.Mint32 st_blk
+        (Ptrofs.unsigned (Ptrofs.repr 44)) Writable). {
+        destruct mperm as (Hrange & _).
+        clear- Hrange.
+        eapply Mem.valid_access_freeable_any; eauto.
+        unfold Mem.valid_access.
+        change (Ptrofs.unsigned (Ptrofs.repr 44)) with 44%Z in *.
+        simpl.
+        split.
+        - unfold Mem.range_perm in *.
+          intros.
+          apply Hrange.
+          lia.
+        - change 44%Z with (4 * 11)%Z.
+          apply Z.divide_factor_l.
+      }
+      eapply Mem.valid_access_store in Heq.
+      destruct Heq as (mk & Heq).
+      exists mk.
+      rewrite Heq; auto.
+    }
+    destruct Hstore_m as (mk & Hstore_m). *)
+    exists Vundef, m', Events.E0.
+
+    unfold stack_block_size in Hbin.
     split.
-    { admit.
+    { eapply Smallstep.star_step with (t1 := Events.E0) (t2 := Events.E0); eauto.
+      { eapply step_seq. }
+      eapply Smallstep.star_step with (t1 := Events.E0) (t2 := Events.E0); eauto.
+      { eapply step_set; forward_expr.
+        - rewrite Ptrofs.add_zero_l.
+          unfold Coqlib.align; simpl.
+          change (Ptrofs.unsigned (Ptrofs.repr (544 / 8))) with
+            (Ptrofs.unsigned (Ptrofs.repr 68)).
+          rewrite Hload_kv.
+          reflexivity.
+        - rewrite Ptrofs.add_zero_l.
+          unfold Coqlib.align; simpl.
+          change (Ptrofs.unsigned (Ptrofs.repr (352 / 8))) with
+            (Ptrofs.unsigned (Ptrofs.repr 44)).
+          rewrite mpc.
+          reflexivity.
+        - unfold Cop.sem_binary_operation, Cop.sem_add; simpl.
+          fold Ptrofs.zero.
+          rewrite Ptrofs.add_zero_l.
+          unfold Coqlib.align; simpl.
+          reflexivity.
+        - unfold Coqlib.align; simpl.
+          change (0 / 8)%Z with 0%Z.
+          fold Ptrofs.zero.
+          rewrite Ptrofs.add_zero.
+          rewrite Hkv1.
+          eapply nth_error_nth with (d := empty_kv) in Hnth.
+          rewrite Hnth.
+          reflexivity.
+      }
+
+      eapply Smallstep.star_step with (t1 := Events.E0) (t2 := Events.E0); eauto.
+      { eapply step_skip_seq. }
+
+      eapply Smallstep.star_step with (t1 := Events.E0) (t2 := Events.E0); eauto.
+      { eapply step_seq. }
+
+      eapply Smallstep.star_step with (t1 := Events.E0) (t2 := Events.E0); eauto.
+      { eapply step_builtin.
+        - econstructor; eauto.
+          { forward_expr.
+            * rewrite Maps.PTree.gso; [ | intro HF; inversion HF].
+              rewrite p0.
+              reflexivity.
+            * rewrite Ptrofs.add_zero_l.
+              unfold Coqlib.align; simpl.
+              change (Ptrofs.unsigned (Ptrofs.repr (608 / 8))) with
+                (Ptrofs.unsigned (Ptrofs.repr 76)).
+              simpl in Hload_bin.
+              rewrite Hload_bin.
+              reflexivity.
+            * rewrite Maps.PTree.gss.
+              reflexivity.
+            * unfold Cop.sem_binary_operation, Cop.sem_add; simpl.
+              fold Ptrofs.zero.
+              rewrite Ptrofs.add_zero_l.
+              reflexivity.
+          }
+          { unfold Cop.sem_cast; simpl.
+            reflexivity. }
+
+          econstructor; eauto.
+          { forward_expr.
+            rewrite Maps.PTree.gso; [ | intro HF; inversion HF].
+            rewrite p0.
+            reflexivity.
+          }
+          { unfold Cop.sem_cast; simpl.
+            reflexivity. }
+
+          econstructor; eauto.
+        - unfold Events.external_call; simpl.
+          split; [reflexivity|].
+          unfold JITTED_LIST_MAX_LENGTH, compcertbin_signature,
+            AST.cc_default, stack_block_size in Hbin1.
+          change (Int.unsigned (Int.repr 48)) with 48%Z in Hbin1.
+          fold Ptrofs.zero.
+          rewrite Heq1, Heq2 in Hbin1.
+          change (Pos.to_nat 4000) with 4000%nat.
+          rewrite Hbin1.
+          reflexivity.
+      }
+
+      eapply Smallstep.star_step with (t1 := Events.E0) (t2 := Events.E0); eauto.
+      { eapply step_skip_seq. }
+
+      eapply Smallstep.star_step with (t1 := Events.E0) (t2 := Events.E0); eauto.
+      { eapply step_seq. }
+
+      clear - Hnth p0 Hst1.
+      destruct Hst1.
+
+
+    simpl in mpc.
+    simpl in mkv.
+    destruct mkv as (Hload_kv & Hkv).
+    unfold match_kv in Hkv.
+    destruct Hkv as (Hkv_len & Hkv_max & Hkv).
+    unfold match_list_kv in Hkv.
+    destruct mbin as (Hload_bin & mbin & Heq1 & Heq2).
+
+    unfold ListKeyV.index in Hnth.
+    specialize (Hkv (Z.to_nat (Int.unsigned ((Int.add (pc_loc st) pc1))))).
+    assert (Hr: (0 <= Z.to_nat (Int.unsigned ((Int.add (pc_loc st) pc1))) < length (tp_kv st))%nat).
+    {
+      clear - Hnth.
+      split; [lia | ].
+      eapply nth_error_Some; eauto.
+      intro HF.
+      rewrite HF in Hnth.
+      inversion Hnth.
+    }
+    specialize (Hkv Hr).
+    destruct Hkv as (Hkv1 & Hkv2).
+    unfold Mem.loadv in Hkv1.
+    assert (Heq:
+    (Ptrofs.unsigned (Ptrofs.repr (8 * Z.of_nat (Z.to_nat (Int.unsigned (pc_loc st)))))) =
+    (Ptrofs.unsigned (Ptrofs.mul (Ptrofs.repr 8) (Ptrofs.of_intu (pc_loc st))))). {
+      clear - Hr.
+      f_equal.
+      unfold Ptrofs.mul, Ptrofs.of_intu, Ptrofs.of_int.
+      f_equal.
+      change (Ptrofs.unsigned (Ptrofs.repr 8)) with 8%Z.
+      rewrite Ptrofs.unsigned_repr_eq.
+      change Ptrofs.modulus with Int.modulus.
+      rewrite <- Int.unsigned_repr_eq.
+      rewrite Int.repr_unsigned.
+      rewrite Z2Nat.id.
+      f_equal.
+      set (Int_unsigned_ge_zero (pc_loc st)) as Heq. lia.
+    }
+    rewrite Heq in Hkv1; clear Heq.
+
+    unfold Mem.loadv in Hkv2.
+    assert (Heq: (Ptrofs.unsigned (Ptrofs.repr (8 * Z.of_nat (Z.to_nat (Int.unsigned (pc_loc st))) + 4))) = (Ptrofs.unsigned
+(Ptrofs.add (Ptrofs.mul (Ptrofs.repr 8) (Ptrofs.of_intu (pc_loc st))) (Ptrofs.repr 4)))). {
+      clear - Hr Hkv_len Hkv_max.
+      f_equal.
+      unfold Ptrofs.add, Ptrofs.mul, Ptrofs.of_intu, Ptrofs.of_int.
+      f_equal.
+      change (Ptrofs.unsigned (Ptrofs.repr 8)) with 8%Z.
+      change (Ptrofs.unsigned (Ptrofs.repr 4)) with 4%Z.
+      repeat rewrite Ptrofs.unsigned_repr_eq.
+      change Ptrofs.modulus with Int.modulus.
+      repeat rewrite <- Int.unsigned_repr_eq.
+      set (Int_unsigned_ge_zero (pc_loc st)) as Heq.
+      rewrite Int.repr_unsigned.
+      rewrite Z2Nat.id; try lia.
+      rewrite Int.unsigned_repr.
+      - f_equal.
+      - change Int.max_unsigned with Ptrofs.max_unsigned.
+          change  Ptrofs.max_unsigned with 4294967295%Z in *.
+          unfold upd_mem, upd_regs, HAVMState.upd_pc in *; simpl in Hkv_max, Hkv_len.
+          rewrite Hkv_len in *.
+          split; lia.
+    }
+    rewrite Heq in Hkv2; clear Heq.
+
+
+
+
+      eapply Smallstep.star_step with (t1 := Events.E0) (t2 := Events.E0); eauto.
+      { repeat (econstructor; eauto; try deref_loc_tactic).
+        - unfold set_opttemp.
+          rewrite Maps.PTree.gso; [| intro HF; inversion HF].
+          eapply p0.
+        - unfold set_opttemp.
+          rewrite Maps.PTree.gso; [| intro HF; inversion HF].
+          eapply p0.
+        - rewrite Ptrofs.add_zero_l.
+          unfold Coqlib.align; simpl.
+          change (Ptrofs.unsigned (Ptrofs.repr (352 / 8))) with
+            (Ptrofs.unsigned (Ptrofs.repr 44)).
+          eapply mpc.
+        - unfold set_opttemp.
+          rewrite Maps.PTree.gso; [| intro HF; inversion HF].
+          eapply p0.
+        - rewrite Ptrofs.add_zero_l.
+          unfold Coqlib.align; simpl.
+          change (Ptrofs.unsigned (Ptrofs.repr (544 / 8))) with
+            (Ptrofs.unsigned (Ptrofs.repr 68)).
+          eapply Hload_kv.
+        - unfold set_opttemp.
+          rewrite Maps.PTree.gso; [| intro HF; inversion HF].
+          eapply p0.
+        - rewrite Ptrofs.add_zero_l.
+          unfold Coqlib.align; simpl.
+          change (Ptrofs.unsigned (Ptrofs.repr (352 / 8))) with
+            (Ptrofs.unsigned (Ptrofs.repr 44)).
+          eapply mpc.
+        - unfold Cop.sem_binary_operation, Cop.sem_add; simpl.
+          fold Ptrofs.zero.
+          rewrite Ptrofs.add_zero_l.
+          unfold Coqlib.align; simpl.
+          reflexivity.
+        - unfold Coqlib.align; simpl.
+          change (32 / 8)%Z with 4%Z.
+          rewrite Hkv2.
+          eapply nth_error_nth with (d := empty_kv) in Hnth.
+          rewrite Hnth.
+          reflexivity.
+
+        - unfold Cop.sem_binary_operation, Cop.sem_add, Cop.sem_binarith; simpl.
+          reflexivity.
+
+        - constructor.
+        - rewrite Ptrofs.add_zero_l.
+          unfold Coqlib.align; simpl.
+          change (Ptrofs.unsigned (Ptrofs.repr (352 / 8))) with
+            (Ptrofs.unsigned (Ptrofs.repr 44)).
+          rewrite Hstore_m.
+          reflexivity.
+      }
+
+      eapply Smallstep.star_step with (t1 := Events.E0) (t2 := Events.E0); eauto.
+      { eapply step_skip_seq. }
+
+      eapply Smallstep.star_step with (t1 := Events.E0) (t2 := Events.E0); eauto.
+      { eapply step_return_0; try reflexivity. }
+      eapply Smallstep.star_refl; eauto.
     }
 
     split_and.
@@ -74,8 +420,16 @@ Definition match_arg_list : DList.t (fun x => x -> Inv _) ((unit:Type) ::args) :
     - unfold upd_regs, upd_mem, HAVMState.upd_pc; simpl.
       inversion MS.
       split; simpl.
-      + eapply Mem.unchanged_on_refl; eauto.
-      + 
+      + eapply rBPFMemType.store_unchanged_on_3; eauto.
+        intros ofs HF.
+        destruct HF as (HF & _).
+        apply HF; reflexivity.
+      + clear - Hcopy_from Hstore_m mregs0.
+        unfold match_registers in *.
+        intros r.
+        specialize (mregs0 r).
+        destruct mregs0 as (vr & Hload_r & Heval_r).
+        
     - simpl; auto.
 Qed.
 
