jit/simulation/correct_jit_call_ax.v
@@ -1,0 +1,48 @@
+From bpf.comm Require Import LemmaInt Regs JITCall.
+From Coq Require Import List Lia ZArith.
+From compcert Require Import Integers Values Clight Memory Memdata.
+Import ListNotations.
+
+From bpf.clightlogic Require Import Clightlogic CorrectRel CommonLemma CommonLib.
+
+From bpf.jit.jitclight Require Import havm_interpreter.
+From bpf.jit Require Import KeyValue2.
+From bpf.jit.havm Require Import HAVMState HAVMMonadOp.
+
+From bpf.jit.simulation Require Import MatchStateComm HAVMMatchState InterpreterRel.
+
+
+Section Jit_call.
+  Context {S : special_blocks}.
+
+  (** The program contains our function of interest [fn] *)
+  Definition p : Clight.program := prog.
+
+  (* [Args,Res] provides the mapping between the Coq and the C types *)
+  (* Definition Args : list CompilableType := [stateCompilableType].*)
+  Definition args : list Type := [].
+  Definition res : Type := unit.
+
+  (* [f] is a Coq Monadic function with the right type *)
+  Definition f : arrow_type args (M res) := jit_call.
+
+  (* [fn] is the Cligth function which has the same behaviour as [f] *)
+  Definition fn: Clight.function := f_jit_call.
+
+  Definition modifies  := ModSomething. (* of the C code *)
+
+  (* [match_arg] relates the Coq arguments and the C arguments *)
+
+
+Definition match_arg_list : DList.t (fun x => x -> Inv _) ((unit:Type) ::args) :=
+    dcons (fun x => StateLess _ (is_state_handle)) (DList.DNil _).
+
+  (* [match_res] relates the Coq result and the C result *)
+  Definition match_res : res -> Inv hybrid_state := fun _  => StateLess _ (fun v => v = Vundef).
+
+
+  Axiom correct_function_jit_call_ax : forall a, correct_function _ p args res f fn modifies false match_state match_arg_list match_res a.
+
+End Jit_call.
+
+Existing Instance correct_function_jit_call_ax.
